src/ListLemmas.v
@@ -371,6 +371,29 @@ eapply Forall2_swap in Hfa.
 fwd eapply Forall2_nth_error_ex; eauto.
 Qed.
 
+Lemma Forall2_imp : forall {A B} (P Q : A -> B -> Prop) xs ys,
+    Forall2 P xs ys ->
+    (forall x y, P x y -> Q x y) ->
+    Forall2 Q xs ys.
+induction xs; destruct ys; intros0 Hfa Himp; invc Hfa; econstructor; eauto.
+Qed.
+
+Lemma Forall2_conj : forall {A B} (P Q : A -> B -> Prop) xs ys,
+    Forall2 P xs ys ->
+    Forall2 Q xs ys ->
+    Forall2 (fun x y => P x y /\ Q x y) xs ys.
+induction xs; destruct ys; intros0 Hfa1 Hfa2; invc Hfa1; invc Hfa2; econstructor; eauto.
+Qed.
+
+Lemma Forall2_conj_inv : forall A B (P Q : A -> B -> Prop) xs ys (M : Prop),
+    (Forall2 P xs ys ->
+        Forall2 Q xs ys ->
+        M) ->
+    Forall2 (fun x y => P x y /\ Q x y) xs ys -> M.
+intros0 HM Hfa.
+eapply HM; eapply Forall2_imp with (1 := Hfa); intros; firstorder.
+Qed.
+
 
 (* misc *)
 
@@ -1537,6 +1560,27 @@ intros.
 erewrite numbered_nth_error_fst;
   eauto using numbered_nth_error_snd.
 Qed.
+
+
+
+
+(* zip *)
+
+Fixpoint zip {A B} (a : list A) (b : list B) : list (A * B) :=
+  match a,b with
+  | f :: r, x :: y => (f,x) :: zip r y
+  | _,_ => nil
+  end.
+
+Lemma zip_nth_error : forall A B (xs : list A) (ys : list B) n xy,
+    nth_error (zip xs ys) n = Some xy ->
+    nth_error xs n = Some (fst xy) /\
+    nth_error ys n = Some (snd xy).
+induction xs; destruct ys, n; intros0 Hzip; simpl in *; try discriminate.
+- inject_some. split; reflexivity.
+- eapply IHxs; eauto.
+Qed.
+
 
 
 
