src/OpaqueTypes.v
@@ -1,4 +1,12 @@
+Require Import compcert.common.AST.
+Require Import compcert.common.Values.
+Require Import compcert.common.Memory.
 Require Import oeuf.SafeInt.
+
+Require Import oeuf.MemInjProps.
+
+Require Import StructTact.StructTactics.
+Require Import oeuf.StuartTact.
 
 Inductive opaque_type_name : Set :=
 | Oint
@@ -23,3 +31,81 @@ destruct oty; simpl in x, y.
 Defined.
 
 
+Record opaque_type_impl {oty} := MkOpaqueTypeImpl {
+    ot_value_inject : opaque_type_denote oty -> val -> mem -> Prop;
+    (* We may eventually need to split this into separate helper lemmas for
+       value_val_inject and value_inject_mem_extends.  Currently we use a
+       slightly weaker precondition in order to use a single helper lemma for
+       both. *)
+    ot_value_val_inject : forall mi m m' cv cv' ov,
+        ot_value_inject ov cv m ->
+        Val.inject mi cv cv' ->
+        Mem.mem_inj mi m m' ->
+        same_offsets mi ->
+        ot_value_inject ov cv' m';
+    ot_inject_defined : forall ov cv m,
+        ot_value_inject ov cv m ->
+        cv <> Vundef;
+    ot_value_32bit : forall ov cv m,
+        ot_value_inject ov cv m ->
+        Val.load_result Mint32 cv = cv
+}.
+
+Implicit Arguments opaque_type_impl [].
+
+
+
+Definition impl_int : opaque_type_impl Oint.
+simple refine (MkOpaqueTypeImpl _  _  _ _ _).
+
+- exact (fun ov cv m => cv = Vint ov).
+
+- intros. simpl in *. on >Val.inject, invc; congruence.
+
+- intros. simpl in *. congruence.
+
+- intros. simpl in *. subst cv. reflexivity.
+Defined.
+
+
+Definition get_opaque_type_impl oty :=
+    match oty with
+    | Oint => impl_int
+    end.
+
+
+
+Section BY_NAME.
+Local Set Implicit Arguments.
+
+Variable oty : opaque_type_name.
+Let impl := get_opaque_type_impl oty.
+
+Definition opaque_type_value_inject := ot_value_inject impl.
+
+Lemma opaque_type_value_val_inject : forall mi m m' cv cv' ov,
+        opaque_type_value_inject ov cv m ->
+        Val.inject mi cv cv' ->
+        Mem.mem_inj mi m m' ->
+        same_offsets mi ->
+        opaque_type_value_inject ov cv' m'.
+intros. unfold opaque_type_value_inject in *.
+eapply (ot_value_val_inject impl); eauto.
+Qed.
+
+Lemma opaque_type_inject_defined : forall ov cv m,
+        opaque_type_value_inject ov cv m ->
+        cv <> Vundef.
+intros. unfold opaque_type_value_inject in *.
+eapply (ot_inject_defined impl); eauto.
+Qed.
+
+Lemma opaque_type_value_32bit : forall ov cv m,
+        opaque_type_value_inject ov cv m ->
+        Val.load_result Mint32 cv = cv.
+intros. unfold opaque_type_value_inject in *.
+eapply (ot_value_32bit impl); eauto.
+Qed.
+
+
+End BY_NAME.
